Establish the standard library location
This commit focuses on clarifying the location to which we extract the
Noir standard library, making it easy to access and work with. In
addition to this, it:

- Clarifies conventions for working with extracted projects.
- Updates all tooling to refer to the new standard library location.
- Establishes the basic skeleton for standard-library proofs, but does
  not include any proofs at this stage.
- Adds steps to CI that check the extracted standard library for
  consistency against the committed version, and also ensures that the
  extracted standard library compiles and tests correctly.

Additionally, it performs a minor version bump to some actions on CI, as
it was already touching the CI configuration.

src/lean/generator.rs
@@ -1308,7 +1308,7 @@ impl LeanGenerator<'_, '_> {
     }
 
     /// Generates the AST for a global definition corresponding to the Noir IR.
-    ///
+    //
     /// # Panics
     ///
     /// - If the global definition pointed to by `id` is malformed.
@@ -1323,13 +1323,7 @@ impl LeanGenerator<'_, '_> {
 
         match statement {
             HirStatement::Let(binding) => {
-                let name = match binding.pattern {
-                    HirPattern::Identifier(hir_ident) => {
-                        self.context.def_interner.definition_name(hir_ident.id).to_string()
-                    }
-                    _ => panic!("Encountered a malformed global"),
-                };
-
+                let name = self.fully_qualified_global_name(id);
                 let typ = self.generate_lean_type_value(&binding.r#type, None);
                 let expr = self.generate_expr(binding.expression);
 
@@ -2225,14 +2219,9 @@ impl LeanGenerator<'_, '_> {
                 let let_stmt = self.context.def_interner.statement(&global_info.let_statement);
                 let (global_name, global_type) = match let_stmt {
                     HirStatement::Let(let_stmt) => {
-                        let ident = match &let_stmt.pattern {
-                            HirPattern::Identifier(hir_ident) => {
-                                self.context.def_interner.definition_name(hir_ident.id).to_string()
-                            }
-                            _ => panic!("Encountered a malformed global"),
-                        };
+                        let name = self.fully_qualified_global_name(id);
                         let typ = self.generate_lean_type_value(&let_stmt.r#type, None);
-                        (ident, typ)
+                        (name, typ)
                     }
                     _ => panic!("Encountered a global that was not defined with a let binding"),
                 };
@@ -2674,6 +2663,56 @@ impl LeanGenerator<'_, '_> {
             format!("std::{fq_name}")
         } else {
             fq_name
+        }
+    }
+
+    /// Returns the fully-qualified global name for the described global.
+    ///
+    /// # Panics
+    ///
+    /// - If the global definition is not a let binding.
+    pub fn fully_qualified_global_name(&self, id: &GlobalId) -> String {
+        let global_data = self.context.def_interner.get_global(*id);
+        let statement = self.context.def_interner.statement(&global_data.let_statement);
+
+        match statement {
+            HirStatement::Let(binding) => match binding.pattern {
+                HirPattern::Identifier(hir_ident) => {
+                    let def_name =
+                        self.context.def_interner.definition_name(hir_ident.id).to_string();
+
+                    let krate = self
+                        .context
+                        .def_map(&global_data.crate_id)
+                        .expect("module should exist in context");
+                    if let Some((id, mod_data)) = krate.modules().iter().find(|(_, m)| {
+                        m.value_definitions()
+                            .any(|i| matches!(i, ModuleDefId::GlobalId(inner) if *id == inner))
+                    }) {
+                        let module_path = krate.get_module_path_with_separator(
+                            LocalModuleId::new(id),
+                            mod_data.parent,
+                            "::",
+                        );
+
+                        if self.root_crate_is_stdlib() {
+                            if module_path.is_empty() {
+                                format!("std::{def_name}")
+                            } else {
+                                format!("std::{module_path}::{def_name}")
+                            }
+                        } else if module_path.is_empty() {
+                            def_name.to_string()
+                        } else {
+                            format!("{module_path}::{def_name}")
+                        }
+                    } else {
+                        def_name.to_string()
+                    }
+                }
+                _ => panic!("Encountered a malformed global"),
+            },
+            _ => panic!("Encountered a malformed global"),
         }
     }
 }
