stdlib/lampe/Stdlib/Option.lean
@@ -1,48 +1,80 @@
-import «std-1.0.0-beta.11».Extracted
--- import «std-1.0.0-beta.11».Extracted.GeneratedTypes
+import «std-1.0.0-beta.11».Extracted.Option
+import «std-1.0.0-beta.11».Extracted.«std-1.0.0-beta.11»
 import Lampe
+
+namespace Lampe
+namespace Stdlib
+
+export «std-1.0.0-beta.11».Extracted (
+  «std::option::Option»
+  «std::option::Option::none»
+  «std::option::Option::some»
+  «std::option::Option::is_none»
+  «std::option::Option::is_some»
+  «std::option::Option::unwrap»
+  «std::option::Option::unwrap_unchecked»
+  «std::option::Option::unwrap_or»
+  «std::option::Option::unwrap_or_else»
+  «std::option::Option::expect»
+  «std::option::Option::map»
+  «std::option::Option::map_or»
+  «std::option::Option::map_or_else»
+  «std::option::Option::and»
+  «std::option::Option::and_then»
+  «std::option::Option::or»
+  «std::option::Option::or_else»
+  «std::option::Option::xor»
+  «std::option::Option::flatten»
+  Option.env
+)
 
 open «std-1.0.0-beta.11».Extracted
 
-#print «struct#std::option::Option»
-
 set_option maxRecDepth 1000
 
-def from_option {p t}: Option (t.denote p) -> («struct#std::option::Option».tp h![t] |>.denote p)
+def from_option {p t}: Option (t.denote p) -> («std::option::Option».tp h![t] |>.denote p)
 | none => (false, Lampe.Tp.zero p t, ())
 | some val => (true, val, ())
 
-def to_option {p t}: («struct#std::option::Option».tp h![t] |>.denote p) -> Option (t.denote p)
+def to_option {p t}: («std::option::Option».tp h![t] |>.denote p) -> Option (t.denote p)
 | (false, _, _) => none
 | (true, val, _) => some val
 
 lemma from_option_to_option_id : to_option (from_option v) = v := by
   cases v <;> rfl
 
-lemma none_spec {p T} : Lampe.STHoare p env ⟦⟧ («std::option::Option::none».call h![T] h![]) (fun v => v = from_option none) := by
+lemma none_spec {p T} : Lampe.STHoare p env ⟦⟧ («std::option::Option::none».call h![T] h![]) 
+    (fun v => v = from_option none) := by
   enter_decl
   steps
   assumption
 
-lemma some_spec {p T v} : Lampe.STHoare p env ⟦⟧ («std::option::Option::some».call h![T] h![v]) (fun r => r = from_option (some v)) := by
+lemma some_spec {p T v} : Lampe.STHoare p env ⟦⟧ («std::option::Option::some».call h![T] h![v])
+    (fun r => r = from_option (some v)) := by
   enter_decl
   steps
   assumption
 
-lemma is_none_spec {p T v} : Lampe.STHoare p env ⟦⟧ («std::option::Option::is_none».call h![T] h![from_option v]) (fun r => r = v.isNone) := by
+lemma is_none_spec {p T v} : Lampe.STHoare p env ⟦⟧ 
+    («std::option::Option::is_none».call h![T] h![from_option v]) 
+    (fun r => r = v.isNone) := by
   enter_decl
   steps
   subst_vars
   cases v <;> rfl
   exact () -- Why?
 
-lemma is_some_spec {p T v} : Lampe.STHoare p env ⟦⟧ («std::option::Option::is_some».call h![T] h![from_option v]) (fun r => r = v.isSome) := by
+lemma is_some_spec {p T v} : Lampe.STHoare p env ⟦⟧ 
+    («std::option::Option::is_some».call h![T] h![from_option v]) 
+    (fun r => r = v.isSome) := by
   enter_decl
   steps
   subst_vars
   cases v <;> rfl
 
-lemma unwrap_spec {p T v} : Lampe.STHoare p env ⟦⟧ («std::option::Option::unwrap».call h![T] h![from_option v]) (fun r => ∃h, r = v.get h) := by
+lemma unwrap_spec {p T v} : Lampe.STHoare p env ⟦⟧ 
+    («std::option::Option::unwrap».call h![T] h![from_option v]) 
+    (fun r => ∃h, r = v.get h) := by
   enter_decl
   steps
   cases v
@@ -53,7 +85,9 @@ lemma unwrap_spec {p T v} : Lampe.STHoare p env ⟦⟧ («std::option::Option::u
     simp
     rfl
 
-lemma map_none_spec {p T U E f} : Lampe.STHoare p env ⟦⟧ («std::option::Option::map».call h![T, U, E] h![from_option none, f]) (fun r => r = from_option (none: Option (U.denote p))) := by
+lemma map_none_spec {p T U E f} : Lampe.STHoare p env ⟦⟧ 
+  («std::option::Option::map».call h![T, U, E] h![from_option none, f]) 
+  (fun r => r = from_option (none: Option (U.denote p))) := by
   enter_decl
   steps
   apply Lampe.STHoare.iteFalse_intro
@@ -79,8 +113,11 @@ lemma map_some_spec {p T U E f fb v P Q}
   sorry -- SL needs work
 
 lemma map_pure_spec {p T U E f fb v f_emb}
-  (h_f: ∀arg, Lampe.STHoare p env ⟦⟧ (fb h![arg]) (fun r => r = f_emb arg)):
-  Lampe.STHoare p env [λf ↦ fb] («std::option::Option::map».call h![T, U, E] h![from_option v, f]) (fun r => r = from_option (v.map f_emb)) := by
+    (h_f: ∀arg, Lampe.STHoare p env ⟦⟧ (fb h![arg]) (fun r => r = f_emb arg)):
+    Lampe.STHoare p env 
+      [λf ↦ fb] 
+      («std::option::Option::map».call h![T, U, E] h![from_option v, f]) 
+      (fun r => r = from_option (v.map f_emb)) := by
   cases v
   · steps [map_none_spec]
     assumption
