stdlib/lampe/Stdlib/Collections/BoundedVec.lean
@@ -1,0 +1,34 @@
+import «std-1.0.0-beta.11».Extracted.Collections.BoundedVec
+import «std-1.0.0-beta.11».Extracted.«std-1.0.0-beta.11»
+import Lampe
+
+namespace Lampe
+namespace Stdlib
+
+export «std-1.0.0-beta.11».Extracted (
+  «std::collections::bounded_vec::BoundedVec»
+  «std::collections::bounded_vec::BoundedVec::new»
+  «std::collections::bounded_vec::BoundedVec::get»
+  «std::collections::bounded_vec::BoundedVec::get_unchecked»
+  «std::collections::bounded_vec::BoundedVec::set»
+  «std::collections::bounded_vec::BoundedVec::set_unchecked»
+  «std::collections::bounded_vec::BoundedVec::push»
+  «std::collections::bounded_vec::BoundedVec::len»
+  «std::collections::bounded_vec::BoundedVec::max_len»
+  «std::collections::bounded_vec::BoundedVec::storage»
+  «std::collections::bounded_vec::BoundedVec::extend_from_array»
+  «std::collections::bounded_vec::BoundedVec::extend_from_slice»
+  «std::collections::bounded_vec::BoundedVec::extend_from_bounded_vec»
+  «std::collections::bounded_vec::BoundedVec::from_array»
+  «std::collections::bounded_vec::BoundedVec::pop»
+  «std::collections::bounded_vec::BoundedVec::any»
+  «std::collections::bounded_vec::BoundedVec::map»
+  «std::collections::bounded_vec::BoundedVec::mapi»
+  «std::collections::bounded_vec::BoundedVec::for_each»
+  «std::collections::bounded_vec::BoundedVec::for_eachi»
+  «std::collections::bounded_vec::BoundedVec::from_parts»
+  «std::collections::bounded_vec::BoundedVec::from_parts_unchecked»
+  Collections.BoundedVec.env
+)
+
+open «std-1.0.0-beta.11».Extracted
