stdlib/lampe/Stdlib/Collections/Vec.lean
@@ -1,0 +1,22 @@
+import «std-1.0.0-beta.11».Extracted.Collections.Vec
+import «std-1.0.0-beta.11».Extracted.«std-1.0.0-beta.11»
+import Lampe
+
+namespace Lampe
+namespace Stdlib
+
+export «std-1.0.0-beta.11».Extracted (
+  «std::collections::vec::Vec»
+  «std::collections::vec::Vec::new»
+  «std::collections::vec::Vec::from_slice»
+  «std::collections::vec::Vec::get»
+  «std::collections::vec::Vec::set»
+  «std::collections::vec::Vec::push»
+  «std::collections::vec::Vec::pop»
+  «std::collections::vec::Vec::insert»
+  «std::collections::vec::Vec::remove»
+  «std::collections::vec::Vec::len»
+  Collections.Vec.env
+)
+
+open «std-1.0.0-beta.11».Extracted
