stdlib/lampe/Stdlib/Hash/Poseidon2.lean
@@ -1,0 +1,19 @@
+import «std-1.0.0-beta.11».Extracted.Hash.Poseidon2
+import «std-1.0.0-beta.11».Extracted.«std-1.0.0-beta.11»
+import Lampe
+
+namespace Lampe
+namespace Stdlib
+
+export «std-1.0.0-beta.11».Extracted (
+  «std::hash::poseidon2::Poseidon2»
+  «std::hash::poseidon2::Poseidon2::hash»
+  «std::hash::poseidon2::Poseidon2::new»
+  «std::hash::poseidon2::Poseidon2::perform_duplex»
+  «std::hash::poseidon2::Poseidon2::absorb»
+  «std::hash::poseidon2::Poseidon2::squeeze»
+  «std::hash::poseidon2::Poseidon2::hash_internal»
+  Hash.Poseidon2.env
+)
+
+open «std-1.0.0-beta.11».Extracted
