stdlib/lampe/Stdlib/Lib.lean
@@ -1,0 +1,22 @@
+import «std-1.0.0-beta.11».Extracted.Lib
+import «std-1.0.0-beta.11».Extracted.«std-1.0.0-beta.11»
+import Lampe
+
+namespace Lampe
+namespace Stdlib
+
+export «std-1.0.0-beta.11».Extracted (
+  «std::print_oracle»
+  «std::print_unconstrained»
+  «std::println»
+  «std::print»
+  «std::verify_proof_with_type»
+  «std::wrapping_add»
+  «std::wrapping_sub»
+  «std::wrapping_mul»
+  «std::tests::test_static_assert_custom_message»
+  «std::tests::test_wrapping_mul»
+  Lib.env
+)
+
+open «std-1.0.0-beta.11».Extracted
