stdlib/lampe/Stdlib/Panic.lean
@@ -1,0 +1,13 @@
+import «std-1.0.0-beta.11».Extracted.Panic
+import «std-1.0.0-beta.11».Extracted.«std-1.0.0-beta.11»
+import Lampe
+
+namespace Lampe
+namespace Stdlib
+
+export «std-1.0.0-beta.11».Extracted (
+  «std::panic::panic»
+  Panic.env
+)
+
+open «std-1.0.0-beta.11».Extracted
